erasure/theories/EOptimizePropDiscr.v
@@ -30,12 +30,6 @@ Hint Constructors eval : core.
 Section optimize.
   Context (Σ : global_context).
 
-  Definition is_box_fix mfix idx := 
-    match nth_error mfix idx with
-    | Some {| dbody := tBox |} => true
-    | _ => false
-    end.
-
   Fixpoint optimize (t : term) : term :=
     match t with
     | tRel i => tRel i
@@ -60,8 +54,7 @@ Section optimize.
       end
     | tFix mfix idx =>
       let mfix' := List.map (map_def optimize) mfix in
-      if is_box_fix mfix idx then tBox
-      else tFix mfix' idx
+      tFix mfix' idx
     | tCoFix mfix idx =>
       let mfix' := List.map (map_def optimize) mfix in
       tCoFix mfix' idx
@@ -128,8 +121,6 @@ Section optimize.
       rtoProp; solve_all. solve_all.
       rtoProp; solve_all. solve_all.
     - destruct EGlobalEnv.inductive_isprop_and_pars as [[[|] _]|]; cbn; auto.
-    - destruct is_box_fix => //.
-      cbn; auto; rewrite forallb_map; len; solve_all.
   Qed.
  
   Lemma subst_csubst_comm l t k b : 
@@ -175,33 +166,16 @@ Section optimize.
   Import EEtaExpanded.
   Ltac solve_discr' := try solve_discr; repeat solve_discr_args; try congruence.
 
-  Lemma optimize_csubst {efl : EEnvFlags} a k i b : 
+  Lemma optimize_csubst a k b : 
     closed a ->
-    wellformed Σ i b ->
     optimize (ECSubst.csubst a k b) = ECSubst.csubst (optimize a) k (optimize b).
   Proof.
-    induction b in i, k |- * using EInduction.term_forall_list_ind; simpl; auto;
-    intros cl exp; try easy; 
+    induction b in k |- * using EInduction.term_forall_list_ind; simpl; auto;
+    intros cl; try easy; 
     rewrite -> ?map_map_compose, ?compose_on_snd, ?compose_map_def, ?map_length;
     unfold test_def in *;
-    simpl closed in *; try solve [depelim exp; try solve_discr'; simpl subst; simpl closed; f_equal; auto; rtoProp; solve_all]; try easy.
+    simpl closed in *; try solve [simpl subst; simpl closed; f_equal; auto; rtoProp; solve_all]; try easy.
     - destruct (k ?= n)%nat; auto.
-    - depelim exp.
-      * destruct args using rev_case; try congruence.
-        rewrite mkApps_app in H2. noconf H2.
-        eapply Forall_app in H1 as []. depelim H2.
-        f_equal; eauto. eapply IHb1; eauto. eapply expanded_mkApps_expanded; eauto; solve_all.
-      * destruct args using rev_case; try congruence. solve_discr.
-        rewrite mkApps_app in H2. noconf H2.
-        eapply Forall_app in H1 as []. depelim H2.
-        rewrite !csubst_mkApps /= !optimize_mkApps /=.
-        rewrite !csubst_mkApps /=. f_equal; eauto. f_equal. solve_all.
-        f_equal; eauto. eapply IHb1; eauto.
-         eapply expanded_mkApps_expanded; eauto; solve_all.
-
-      *
-         eauto.
-      eapply IHb1. auto.
     - unfold on_snd; cbn.
       destruct EGlobalEnv.inductive_isprop_and_pars as [[[|] _]|] => /= //.
       destruct l as [|[br n] [|l']] eqn:eql; simpl.
@@ -209,7 +183,7 @@ Section optimize.
       * depelim X. simpl in *.
         rewrite e //.
         assert (#|br| = #|repeat tBox #|br| |). now rewrite repeat_length.
-        rewrite {2}H0.
+        rewrite {2}H.
         rewrite substl_csubst_comm //.
         solve_all. eapply All_repeat => //.
         now eapply closed_optimize.
@@ -222,9 +196,6 @@ Section optimize.
       * rewrite ?map_map_compose; f_equal; eauto; solve_all.
     - destruct EGlobalEnv.inductive_isprop_and_pars as [[[|] _]|]=> //;
       now rewrite IHb.
-    - rewrite  !nth_error_map.
-      destruct nth_error => /= //.
-
   Qed.
 
   Lemma optimize_substl s t : 
@@ -714,8 +685,7 @@ Proof.
     destruct inductive_isprop_and_pars as [[[|] _]|] => /= //.
     constructor. all:constructor; auto.
   - cbn. eapply expanded_tFix. solve_all.
-    rewrite isLambda_optimize //. now left.
-    rewrite isBox_optimize //. now right.
+    rewrite isLambda_optimize //.
   - eapply expanded_tConstruct_app; tea.
     now len. solve_all.
 Qed.
